omnibig

omni/OmniBig.v
@@ -3,49 +3,31 @@
 * Omni-Big-Step Semantics                                       *
 *****************************************************************)
 
+Set Implicit Arguments.
+Require Export Big.
+
+Implicit Types f : var.
+Implicit Types b : bool.
+Implicit Types p : loc.
+Implicit Types n : int.
+Implicit Types v w r vf vx : val.
+Implicit Types t : trm.
+Implicit Types s : state.
+
+Implicit Types P : state->trm->Prop.
+Implicit Types Q : val->state->Prop.
 
 
 (* ########################################################### *)
 (* ########################################################### *)
 (* ########################################################### *)
-(** * Common definitions  *)
+(** * Definitions  *)
 
 (* ########################################################### *)
-(** ** Definition of [strongestpost] and [exactly] *)
+(** ** Inductive Omni-Big-Step *)
 
-(** Let [strongestpost s t] denote the strongest postcondition
-    (strongest-post), that is, [fun v s' => big s t s' v]. *)
-
-Definition strongestpost (s:state) (t:trm) : val->hprop :=
-  fun v s' => big s t s' v.
-
-(* The postcondition [exactly v s'] to assert that the output of a program
-   is exactly the value [v] in the state [s']. This postcondition
-   corresponds to a singleton set. *)
-
-Definition exactly (v:val) (s':state) : val->hprop :=
-  fun v0 s0 => v0 = v /\ s0 = s'.
-
-(** By definition, the postcondition [exactly v s'] holds only of [v]
-    and [s'], thus the only introduction rule for [exactly] is the
-    following reflexivity rule. *)
-
-Lemma exactly_intro : forall v s',
-  exactly v s' v s'.
-Proof using. intros. hnfs*. Qed.
-
-
-
-
-(* ########################################################### *)
-(* ########################################################### *)
-(* ########################################################### *)
-(** * Inductive Omni-Big-Step *)
-
-(* ########################################################### *)
-(** ** Definition of Omni-Big-Step *)
-
-(** Judgment [omnibig s t Q] *)
+(** The judgment [omnibig s t Q] asserts that all executions starting from [(s,t)]
+    eventually reach a final configuration satisfying the predicate [Q]. *)
 
 Inductive omnibig : state -> trm -> (val->state->Prop) -> Prop :=
   | omnibig_val : forall s v Q,
@@ -90,326 +72,9 @@ Inductive omnibig : state -> trm -> (val->state->Prop) -> Prop :=
       Q val_unit (Fmap.remove s p) ->
       omnibig s (val_free (val_loc p)) Q.
 
-(** [omnibig] is covariant in the postcondition (omni-big-conseqence) *)
-
-Lemma omnibig_conseq : forall s t Q1 Q2,
-  omnibig s t Q1 ->
-  Q1 ===> Q2 ->
-  omnibig s t Q2.
-Proof using.
-  introv M W.
-  asserts W': (forall v h, Q1 v h -> Q2 v h). { auto. } clear W.
-  induction M; try solve [ constructors* ].
-Qed.
-
 
 (* ########################################################### *)
-(** ** Relationship with WP Formulation *)
-
-(** The rule [omnibig_let] shares similarities with the statement of
-    the weakest-precondition style reasoning rule for let-bindings.
-    Prove the following alternative statement, with a wp-style flavor. *)
-
-Lemma omnibig_let' : forall s1 x t1 t2 Q,
-  omnibig s1 t1 (fun v1 s2 => omnibig s2 (subst x v1 t2) Q) ->
-  omnibig s1 (trm_let x t1 t2) Q.
-Proof using.
-  introv M. applys* omnibig_let M.
-Qed.
-
-(** Reciprocally, prove that the statement considered in the inductive
-    definition of [omnibig] is derivable from [omnibig_let']. More precisely,
-    prove the statement below by using [omnibig_let'] and [omnibig_conseq]. *)
-
-Lemma omnibig_let_of_omnibig_let' : forall Q1 s1 x t1 t2 Q,
-  omnibig s1 t1 Q1 ->
-  (forall v1 s2, Q1 v1 s2 -> omnibig s2 (subst x v1 t2) Q) ->
-  omnibig s1 (trm_let x t1 t2) Q.
-Proof using.
-  introv M1 M2. applys omnibig_let'. applys omnibig_conseq M1.
-  intros v1 s2 K. applys M2 K.
-Qed.
-
-(** One way wonder whether we could have used the wp-style formulation
-    of the semantics of let-bindings directly in the definition of [omnibig].
-    The answer is negative. Doing so would lead to an invalid inductive
-    definition, involving a "non strictly positive occurrence". To check it
-    out, uncomment the definitions below to observe Coq's complaint.
-[[
-  Inductive omnibig' : state -> trm -> (val->state->Prop) -> Prop :=
-    | omnibig'_let : forall s1 x t1 t2 Q,
-       omnibig' s1 t1 (fun v1 s2 => omnibig' s2 (subst x v1 t2) Q) ->
-       omnibig' s1 (trm_let x t1 t2) Q.
-
-  Inductive omnibig' : state -> trm -> (val->state->Prop) -> Prop :=
-    | omnibig'_let : forall Q1 s1 x t1 t2 Q,
-       omnibig' s1 t1 Q1 ->
-       Q1 = (fun v1 s2 => omnibig' s2 (subst x v1 t2) Q) ->
-       omnibig' s1 (trm_let x t1 t2) Q.
-]]
-
-   Yet another unsuccessful try:
-[[
-  Inductive omnibig' : state -> trm -> (val->state->Prop) -> Prop :=
-    | omnibig'_let : forall Q1 s1 x t1 t2 Q,
-       omnibig' s1 t1 Q1 ->
-       (forall v1 s2, Q1 v1 s2 -> exists Q2, omnibig' s2 (subst x v1 t2) Q2) ->
-       Q = (fun v2 s3 => exists v1 s2, Q1 v1 s2 /\ exists Q2, Q2 v2 s3 /\ omnibig' s2 (subst x v1 t2) Q2) ->
-       omnibig' s1 (trm_let x t1 t2) Q.
-]]
-*)
-
-
-(* ########################################################### *)
-(** ** Properties of Omni-Big-Step, Part 1 *)
-
-(** Assume [omnibig s t Q] to hold. Prove that the postcondition [Q] holds of
-    any output that [(s,t)] may evaluate to according to the judgment [big]. *)
-
-Lemma omnibig_and_big_inv : forall s t v s' Q,
-  omnibig s t Q ->
-  big s t s' v ->
-  Q v s'.
-Proof using.
-  introv M R. gen v s'.
-  induction M; intros; try solve [inverts* R; tryfalse].
-  { invert R; try solve [intros; false].
-    introv E R. intros. subst. inverts E. applys* IHM. }
-Qed.
-
-(** If [omnibig s t Q] holds, then there exists an output
-    [(s',v)] that [(s,t)] may evaluate to according to the judgment
-    [big], and that this output satisfies [Q]. *)
-
-Lemma omnibig_to_one_big : forall s t Q,
-  omnibig s t Q ->
-  exists s' v, big s t s' v /\ Q v s'.
-Proof using.
-  introv M. cuts (s'&v&R): (exists s' v, big s t s' v).
-  { exists. split. { applys R. } { applys omnibig_and_big_inv M R. } }
-  induction M.
-  { exists. applys big_val. }
-  { exists. applys big_fix. }
-  { rename IHM into IHM1, M into M1.
-    forwards (s'&v&R): IHM1.
-    exists. applys* big_app_fix R. }
-  { rename IHM into IHM1, H0 into IHM2, M into M1, H into M2.
-    forwards (s1'&v1&R1): IHM1.
-    lets HQ1: omnibig_and_big_inv M1 R1.
-    forwards (s'&v&R2): IHM2 HQ1.
-    exists. applys big_let R1 R2. }
-  { forwards (s'&v&R1): IHM.
-    exists. applys* big_if R1. }
-  { exists. applys* big_div. }
-  { rename H0 into N.
-    exists. applys* big_rand 0. math. }
-  { forwards* (p&D&N): (exists_fresh null s).
-    exists. applys* big_ref. }
-  { exists. applys* big_get. }
-  { exists. applys* big_set. }
-  { exists. applys* big_free. }
-Qed.
-
-
-(* ########################################################### *)
-(** ** Properties of Omni-Big-Step, Part 2 *)
-
-(** A special case is that of programs that admit a unique possible
-    execution, that is, of programs that are deterministic even though
-    the host language includes potentially non-deterministic features.
-    Such a deterministic program admits a unique output. *)
-
-(** A program [(s,t)] admits a unique execution with [(s',v)] as output
-    if and only if [omnibig s t (exactly s' v)] holds. This same property
-    can be expressed in terms of the judgment [big], by asserting that
-    [big s t v2 s2] holds if and only if [v2 = v] and [s2 = s']. Let us
-    prove the two characterizations equivalent. *)
-
-(** We prove that if [omnibig s t Q] holds for a singleton set [Q],
-    then the big-step judgment holds for that unique result. *)
-
-Lemma big_of_omnibig_exactly : forall s t v s',
-  omnibig s t (exactly v s') ->
-  big s t s' v.
-Proof using.
-  introv M. lets (s2&v2&R&E): omnibig_to_one_big M.
-  unfolds exactly. destruct E as (->&->). applys R.
-Qed.
-
-(** A slightly stronger result, not needed in the other proofs. *)
-
-Lemma evalntb_exactly_iff_big_exactly : forall s t v s',
-  omnibig s t (exactly v s') ->
-  (forall s2 v2, big s t s2 v2 <-> (v2 = v /\ s2 = s')).
-Proof using.
-  introv M. iff R (->&->).
-  { applys omnibig_and_big_inv M R. }
-  { lets (s2&v2&R&E): omnibig_to_one_big M.
-    unfolds exactly. destruct E as (->&->). applys R. }
-Qed.
-
-
-(* ########################################################### *)
-(** ** Properties of Omni-Big-Step, Part 3 *)
-
-(** If [omnibig s t Q] holds for some [Q], then
-    [omnibig s t (strongestpost s t)] holds.
-    See also lemma [omnibig_strongestpost_of_terminates]. *)
-
-Lemma omnibig_strongestpost_of_omnibig : forall s t Q,
-  omnibig s t Q ->
-  omnibig s t (strongestpost s t).
-Proof using.
-  introv M. unfold strongestpost. induction M.
-  { applys omnibig_val. applys big_val. }
-  { applys omnibig_fix. applys big_fix. }
-  { applys* omnibig_app_fix. applys omnibig_conseq IHM.
-    { intros v s' R. applys* big_app_fix R. } }
-  { rename IHM into IHM1, H0 into IHM2.
-    applys omnibig_let (fun v1 s' => big s t1 s' v1 /\ Q1 v1 s').
-    { applys omnibig_conseq IHM1. { intros v1 s' R. split.
-      { applys R. }
-      { applys omnibig_and_big_inv M R. } } }
-    { intros v1 s2 (R1&K). applys omnibig_conseq. applys IHM2 K.
-      { intros v s' R2. applys big_let R1 R2. } } }
-  { applys omnibig_if. applys omnibig_conseq IHM.
-    { intros v s' R. applys big_if R. } }
-  { applys omnibig_div. applys big_div. }
-  { applys* omnibig_rand. intros n1 N1. applys* big_rand. }
-  { applys* omnibig_ref. intros p Hp. applys* big_ref. }
-  { applys* omnibig_get. applys* big_get. }
-  { applys* omnibig_set. applys* big_set. }
-  { applys* omnibig_free. applys* big_free. }
-Qed.
-
-(** Reciprocally, the strongest postcondition is the smallest
-    possible postcondition for the judgment (strongest-post-minimal). *)
-
-Lemma omnibig_inv_strongestpost_qimpl : forall s t Q,
-  omnibig s t Q ->
-  strongestpost s t ===> Q.
-Proof using.
-  introv M. unfold strongestpost. intros v s' K. applys omnibig_and_big_inv M K.
-Qed.
-
-
-(* ########################################################### *)
-(** ** Interpretation of Omni-Big-Step w.r.t. [terminates] *)
-
-(** The predicate [terminates s t] asserts that all executions of the
-    configuration [t/s] terminate---none of them diverges or get
-    stuck. Its definition is a simplified version of [omnibig] where all
-    occurences of [Q] are removed. In the rule for let-bindings,
-    namely [terminates_let], the quantification over the configuration
-    [v1/s2] is done by refering to the big-step judgment [big]. *)
-
-Inductive terminates : state -> trm -> Prop :=
-  | terminates_val : forall s v,
-      terminates s (trm_val v)
-  | terminates_fix : forall s f x t1,
-      terminates s (trm_fix f x t1)
-  | terminates_app_fix : forall s v1 v2 f x t1,
-      v1 = val_fix f x t1 ->
-      terminates s (subst x v2 (subst f v1 t1)) ->
-      terminates s (trm_app v1 v2)
-  | terminates_let : forall s x t1 t2,
-      terminates s t1 ->
-      (forall v1 s2, big s t1 s2 v1 -> terminates s2 (subst x v1 t2)) ->
-      terminates s (trm_let x t1 t2)
-  | terminates_if : forall s b t1 t2,
-      terminates s (if b then t1 else t2) ->
-      terminates s (trm_if (val_bool b) t1 t2)
-  | terminatess_div : forall s n1 n2,
-      n2 <> 0 ->
-      terminates s (val_div (val_int n1) (val_int n2))
-  | terminates_rand : forall s n,
-      n > 0 ->
-      terminates s (val_rand (val_int n))
-  | terminates_ref : forall s v,
-      terminates s (val_ref v)
-  | terminates_get : forall s p,
-      Fmap.indom s p ->
-      terminates s (val_get (val_loc p))
-  | terminates_set : forall s p v,
-      Fmap.indom s p ->
-      terminates s (val_set (val_loc p) v)
-  | terminates_free : forall s p,
-      Fmap.indom s p ->
-      terminates s (val_free (val_loc p)).
-
-Section OmnibitTerminates.
-Hint Constructors big omnibig.
-
-(** We prove that [omnibig s t Q] is equivalent to the conjunction of
-    [terminates s t] and to a partial correctness result asserting that
-    if an evaluation of [t/s] terminates on some result then this result
-    satisfies [Q]. (omni-big-step-iff-terminates-and-correct) *)
-
-Lemma omnibig_iff_terminates_and_post : forall s t Q,
-  omnibig s t Q <-> (terminates s t /\ (forall v s', big s t s' v -> Q v s')).
-Proof using.
-  iff M.
-  { split.
-    { induction M; try solve [constructors*].
-      { rename M into M1, H into M2, IHM into IH1, H0 into IH2.
-        constructors.
-        { applys IH1. }
-        { introv R. applys IH2. applys omnibig_and_big_inv M1 R. } } }
-    { introv R. applys omnibig_and_big_inv M R. } }
-  { destruct M as (HS&HQ). gen Q.
-    induction HS; try solve [constructors*].
-    { rename HS into M1, H into M2, IHHS into IH1, H0 into IH2.
-      intros Q HQ.
-      applys omnibig_let (fun v1 s2 => big s t1 s2 v1).
-      { applys* IH1. }
-      { introv R1. applys IH2.
-        { applys R1. }
-        { introv R2. applys* HQ. } } } }
-Qed.
-
-(** We prove that [terminates s t] is equivalent to [omnibig s t Any]. *)
-
-Lemma terminates_iff_omnibig_any : forall s t,
-  terminates s t <-> omnibig s t Any.
-Proof using.
-  intros. rewrite* (omnibig_iff_terminates_and_post s t Any).
-Qed.
-
-End OmnibitTerminates.
-
-(** We can reformulate the right to left direction of
-    [terminates_iff_omnibig_any] by stating that if [omnibig]
-    holds for some [Q], then [terminates s t] holds. *)
-
-Lemma terminates_of_omnibig : forall s t Q,
-  omnibig s t Q ->
-  terminates s t.
-Proof using.
-  introv M. rewrite terminates_iff_omnibig_any.
-  applys omnibig_conseq M. intros s' v. auto.
-Qed.
-
-(** We can reformulate [omnibig_strongestpost_of_omnibig]
-    with [terminates] as premise. (strongest-post-correct) *)
-
-Lemma omnibig_strongestpost_of_terminates : forall s t,
-  terminates s t ->
-  omnibig s t (strongestpost s t).
-Proof using.
-  introv M. rewrite terminates_iff_omnibig_any in M.
-  applys omnibig_strongestpost_of_omnibig M.
-Qed.
-
-
-
-
-(* ########################################################### *)
-(* ########################################################### *)
-(* ########################################################### *)
-(** * Coinductive Omni-big-step *)
-
-(* ########################################################### *)
-(** ** Definition of Coinductive Omni-Big-Step *)
+(** ** Coinductive Omni-Big-Step *)
 
 (** The definition of the predicate [coomnibig] is obtained by taking the
     constructors from the inductive definition of [steps], and considering
@@ -461,7 +126,364 @@ CoInductive coomnibig : state -> trm -> (val->state->Prop) -> Prop :=
       Q val_unit (Fmap.remove s p) ->
       coomnibig s (val_free (val_loc p)) Q.
 
-(** Covariance property. *)
+
+(* ########################################################### *)
+(** ** Omni-Big-Step-Style Inductive Definition of Termination *)
+
+(** The predicate [bigterminates s t] asserts that all executions of the
+    configuration [t/s] terminate---none of them diverges or get
+    stuck. Its definition is a simplified version of [omnibig] where all
+    occurences of [Q] are removed. In the rule for let-bindings,
+    namely [bigterminates_let], the quantification over the configuration
+    [v1/s2] is done by refering to the big-step judgment [big]. *)
+
+Inductive bigterminates : state -> trm -> Prop :=
+  | bigterminates_val : forall s v,
+      bigterminates s (trm_val v)
+  | bigterminates_fix : forall s f x t1,
+      bigterminates s (trm_fix f x t1)
+  | bigterminates_app_fix : forall s v1 v2 f x t1,
+      v1 = val_fix f x t1 ->
+      bigterminates s (subst x v2 (subst f v1 t1)) ->
+      bigterminates s (trm_app v1 v2)
+  | bigterminates_let : forall s x t1 t2,
+      bigterminates s t1 ->
+      (forall v1 s2, big s t1 s2 v1 -> bigterminates s2 (subst x v1 t2)) ->
+      bigterminates s (trm_let x t1 t2)
+  | bigterminates_if : forall s b t1 t2,
+      bigterminates s (if b then t1 else t2) ->
+      bigterminates s (trm_if (val_bool b) t1 t2)
+  | bigterminatess_div : forall s n1 n2,
+      n2 <> 0 ->
+      bigterminates s (val_div (val_int n1) (val_int n2))
+  | bigterminates_rand : forall s n,
+      n > 0 ->
+      bigterminates s (val_rand (val_int n))
+  | bigterminates_ref : forall s v,
+      bigterminates s (val_ref v)
+  | bigterminates_get : forall s p,
+      Fmap.indom s p ->
+      bigterminates s (val_get (val_loc p))
+  | bigterminates_set : forall s p v,
+      Fmap.indom s p ->
+      bigterminates s (val_set (val_loc p) v)
+  | bigterminates_free : forall s p,
+      Fmap.indom s p ->
+      bigterminates s (val_free (val_loc p)).
+
+
+(* ########################################################### *)
+(** ** Omni-Big-Step-Style CoInductive Definition of Safety *)
+
+(** The predicate [bigsafe s t] asserts that an execution of the configuration
+    [t/s] can never get stuck. Its definition is a simplified version of
+    [coomnibig] where all occurences of [Q] are removed. In the rule for let-
+    bindings, namely [bigsafe_let], the quantification over the configuration
+    [v1/s2] is done by refering to the big-step judgment [eval]. *)
+
+CoInductive bigsafe : state -> trm -> Prop :=
+  | bigsafe_val : forall s v,
+      bigsafe s (trm_val v)
+  | bigsafe_fix : forall s f x t1,
+      bigsafe s (trm_fix f x t1)
+  | bigsafe_app_fix : forall s v1 v2 f x t1,
+      v1 = val_fix f x t1 ->
+      bigsafe s (subst x v2 (subst f v1 t1)) ->
+      bigsafe s (trm_app v1 v2)
+  | bigsafe_let : forall s x t1 t2,
+      bigsafe s t1 ->
+      (forall v1 s2, big s t1 s2 v1 -> bigsafe s2 (subst x v1 t2)) ->
+      bigsafe s (trm_let x t1 t2)
+  | bigsafe_if : forall s b t1 t2,
+      bigsafe s (if b then t1 else t2) ->
+      bigsafe s (trm_if (val_bool b) t1 t2)
+  | bigsafes_div : forall s n1 n2,
+      n2 <> 0 ->
+      bigsafe s (val_div (val_int n1) (val_int n2))
+  | bigsafe_rand : forall s n,
+      n > 0 ->
+      bigsafe s (val_rand (val_int n))
+  | bigsafe_ref : forall s v,
+      bigsafe s (val_ref v)
+  | bigsafe_get : forall s p,
+      Fmap.indom s p ->
+      bigsafe s (val_get (val_loc p))
+  | bigsafe_set : forall s p v,
+      Fmap.indom s p ->
+      bigsafe s (val_set (val_loc p) v)
+  | bigsafe_free : forall s p,
+      Fmap.indom s p ->
+      bigsafe s (val_free (val_loc p)).
+
+
+(* ########################################################### *)
+(** ** Omni-Big-Step Divergence *)
+
+(** The judgment [coomnidiv s t] asserts that every possible
+    execution of the program [(s,t)] diverges. It is defined
+    in terms of the coinductive Omni-Big-Step judgment.
+    [Empty] is defined in the file [Syntax]. *)
+
+Definition coomnidiv (s:state) (t:trm) : Prop :=
+  coomnibig s t Empty.
+
+
+(* ########################################################### *)
+(** ** Definition of [strongestpost] and [exactly] *)
+
+(** Let [strongestpost s t] denote the strongest postcondition
+    (strongest-post), that is, [fun v s' => big s t s' v]. *)
+
+Definition strongestpost (s:state) (t:trm) : val->hprop :=
+  fun v s' => big s t s' v.
+
+(* The postcondition [exactly v s'] to assert that the output of a program
+   is exactly the value [v] in the state [s']. This postcondition
+   corresponds to a singleton set. *)
+
+Definition exactly (v:val) (s':state) : val->hprop :=
+  fun v0 s0 => v0 = v /\ s0 = s'.
+
+
+(* ########################################################### *)
+(* ########################################################### *)
+(* ########################################################### *)
+(** * Properties  *)
+
+(* ########################################################### *)
+(** ** Properties of [exactly] *)
+
+(** By definition, the postcondition [exactly v s'] holds only of [v]
+    and [s'], thus the only introduction rule for [exactly] is the
+    following reflexivity rule. *)
+
+Lemma exactly_intro : forall v s',
+  exactly v s' v s'.
+Proof using. intros. hnfs*. Qed.
+
+
+(* ########################################################### *)
+(** ** Properties of [omnibig] *)
+
+(** [omnibig] is covariant in the postcondition (omni-big-conseqence) *)
+
+Lemma omnibig_conseq : forall s t Q1 Q2,
+  omnibig s t Q1 ->
+  Q1 ===> Q2 ->
+  omnibig s t Q2.
+Proof using.
+  introv M W.
+  asserts W': (forall v h, Q1 v h -> Q2 v h). { auto. } clear W.
+  induction M; try solve [ constructors* ].
+Qed.
+
+(** Assume [omnibig s t Q] to hold. Prove that the postcondition [Q] holds of
+    any output that [(s,t)] may evaluate to according to the judgment [big]. *)
+
+Lemma omnibig_and_big_inv : forall s t v s' Q,
+  omnibig s t Q ->
+  big s t s' v ->
+  Q v s'.
+Proof using.
+  introv M R. gen v s'.
+  induction M; intros; try solve [inverts* R; tryfalse].
+  { invert R; try solve [intros; false].
+    introv E R. intros. subst. inverts E. applys* IHM. }
+Qed.
+
+(** If [omnibig s t Q] holds, then there exists an output
+    [(s',v)] that [(s,t)] may evaluate to according to the judgment
+    [big], and that this output satisfies [Q]. *)
+
+Lemma omnibig_to_one_big : forall s t Q,
+  omnibig s t Q ->
+  exists s' v, big s t s' v /\ Q v s'.
+Proof using.
+  introv M. cuts (s'&v&R): (exists s' v, big s t s' v).
+  { exists. split. { applys R. } { applys omnibig_and_big_inv M R. } }
+  induction M.
+  { exists. applys big_val. }
+  { exists. applys big_fix. }
+  { rename IHM into IHM1, M into M1.
+    forwards (s'&v&R): IHM1.
+    exists. applys* big_app_fix R. }
+  { rename IHM into IHM1, H0 into IHM2, M into M1, H into M2.
+    forwards (s1'&v1&R1): IHM1.
+    lets HQ1: omnibig_and_big_inv M1 R1.
+    forwards (s'&v&R2): IHM2 HQ1.
+    exists. applys big_let R1 R2. }
+  { forwards (s'&v&R1): IHM.
+    exists. applys* big_if R1. }
+  { exists. applys* big_div. }
+  { rename H0 into N.
+    exists. applys* big_rand 0. math. }
+  { forwards* (p&D&N): (exists_fresh null s).
+    exists. applys* big_ref. }
+  { exists. applys* big_get. }
+  { exists. applys* big_set. }
+  { exists. applys* big_free. }
+Qed.
+
+(** If [omnibig s t Q] holds for some [Q], then
+    [omnibig s t (strongestpost s t)] holds.
+    See also lemma [omnibig_strongestpost_of_bigterminates]. *)
+
+Lemma omnibig_strongestpost_of_omnibig : forall s t Q,
+  omnibig s t Q ->
+  omnibig s t (strongestpost s t).
+Proof using.
+  introv M. unfold strongestpost. induction M.
+  { applys omnibig_val. applys big_val. }
+  { applys omnibig_fix. applys big_fix. }
+  { applys* omnibig_app_fix. applys omnibig_conseq IHM.
+    { intros v s' R. applys* big_app_fix R. } }
+  { rename IHM into IHM1, H0 into IHM2.
+    applys omnibig_let (fun v1 s' => big s t1 s' v1 /\ Q1 v1 s').
+    { applys omnibig_conseq IHM1. { intros v1 s' R. split.
+      { applys R. }
+      { applys omnibig_and_big_inv M R. } } }
+    { intros v1 s2 (R1&K). applys omnibig_conseq. applys IHM2 K.
+      { intros v s' R2. applys big_let R1 R2. } } }
+  { applys omnibig_if. applys omnibig_conseq IHM.
+    { intros v s' R. applys big_if R. } }
+  { applys* omnibig_div. applys big_div. }
+  { applys* omnibig_rand. intros n1 N1. applys* big_rand. }
+  { applys* omnibig_ref. intros p Hp. applys* big_ref. }
+  { applys* omnibig_get. applys* big_get. }
+  { applys* omnibig_set. applys* big_set. }
+  { applys* omnibig_free. applys* big_free. }
+Qed.
+
+(** Reciprocally, the strongest postcondition is the smallest
+    possible postcondition for the judgment (strongest-post-minimal). *)
+
+Lemma omnibig_inv_strongestpost_qimpl : forall s t Q,
+  omnibig s t Q ->
+  strongestpost s t ===> Q.
+Proof using.
+  introv M. unfold strongestpost. intros v s' K. applys omnibig_and_big_inv M K.
+Qed.
+
+Section OmnibitTerminates.
+Hint Constructors big omnibig.
+
+(** We prove that [omnibig s t Q] is equivalent to the conjunction of
+    [bigterminates s t] and to a partial correctness result asserting that
+    if an evaluation of [t/s] bigterminates on some result then this result
+    satisfies [Q]. (omni-big-step-iff-bigterminates-and-correct) *)
+
+Lemma omnibig_iff_bigterminates_and_post : forall s t Q,
+  omnibig s t Q <-> (bigterminates s t /\ (forall v s', big s t s' v -> Q v s')).
+Proof using.
+  iff M.
+  { split.
+    { induction M; try solve [constructors*].
+      { rename M into M1, H into M2, IHM into IH1, H0 into IH2.
+        constructors.
+        { applys IH1. }
+        { introv R. applys IH2. applys omnibig_and_big_inv M1 R. } } }
+    { introv R. applys omnibig_and_big_inv M R. } }
+  { destruct M as (HS&HQ). gen Q.
+    induction HS; try solve [constructors*].
+    { rename HS into M1, H into M2, IHHS into IH1, H0 into IH2.
+      intros Q HQ.
+      applys omnibig_let (fun v1 s2 => big s t1 s2 v1).
+      { applys* IH1. }
+      { introv R1. applys IH2.
+        { applys R1. }
+        { introv R2. applys* HQ. } } } }
+Qed.
+
+(** We prove that [bigterminates s t] is equivalent to [omnibig s t Any]. *)
+
+Lemma bigterminates_iff_omnibig_any : forall s t,
+  bigterminates s t <-> omnibig s t Any.
+Proof using.
+  intros. rewrite* (omnibig_iff_bigterminates_and_post s t Any).
+Qed.
+
+End OmnibitTerminates.
+
+(** We can reformulate the right to left direction of
+    [bigterminates_iff_omnibig_any] by stating that if [omnibig]
+    holds for some [Q], then [bigterminates s t] holds. *)
+
+Lemma bigterminates_of_omnibig : forall s t Q,
+  omnibig s t Q ->
+  bigterminates s t.
+Proof using.
+  introv M. rewrite bigterminates_iff_omnibig_any.
+  applys omnibig_conseq M. intros s' v. auto.
+Qed.
+
+(** We can reformulate [omnibig_strongestpost_of_omnibig]
+    with [bigterminates] as premise. (strongest-post-correct) *)
+
+Lemma omnibig_strongestpost_of_bigterminates : forall s t,
+  bigterminates s t ->
+  omnibig s t (strongestpost s t).
+Proof using.
+  introv M. rewrite bigterminates_iff_omnibig_any in M.
+  applys omnibig_strongestpost_of_omnibig M.
+Qed.
+
+
+(* ########################################################### *)
+(** ** Properties of Omni-Big-Step for Single-Output Executions *)
+
+(** A special case is that of programs that admit a unique possible
+    execution, that is, of programs that are deterministic even though
+    the host language includes potentially non-deterministic features.
+    Such a deterministic program admits a unique output. *)
+
+(** A program [(s,t)] admits a unique execution with [(s',v)] as output
+    if and only if [omnibig s t (exactly s' v)] holds. This same property
+    can be expressed in terms of the judgment [big], by asserting that
+    [big s t v2 s2] holds if and only if [v2 = v] and [s2 = s']. Let us
+    prove the two characterizations equivalent. *)
+
+(** We prove that if [omnibig s t Q] holds for a singleton set [Q],
+    then the big-step judgment holds for that unique result. *)
+
+Lemma big_of_omnibig_exactly : forall s t v s',
+  omnibig s t (exactly v s') ->
+  big s t s' v.
+Proof using.
+  introv M. lets (s2&v2&R&E): omnibig_to_one_big M.
+  unfolds exactly. destruct E as (->&->). applys R.
+Qed.
+
+(** A slightly stronger result, not needed in the other proofs. *)
+
+Lemma evalntb_exactly_iff_big_exactly : forall s t v s',
+  omnibig s t (exactly v s') ->
+  (forall s2 v2, big s t s2 v2 <-> (v2 = v /\ s2 = s')).
+Proof using.
+  introv M. iff R (->&->).
+  { applys omnibig_and_big_inv M R. }
+  { lets (s2&v2&R&E): omnibig_to_one_big M.
+    unfolds exactly. destruct E as (->&->). applys R. }
+Qed.
+
+
+(* ########################################################### *)
+(** ** Total Correctness Entails Partial Correctness *)
+
+(** Total correctness is a stronger property than partial correctness:
+    [omnibig s t Q] entails [coomnibig s t Q]. *)
+
+Lemma coomnibig_of_omnibig : forall s t Q,
+  omnibig s t Q ->
+  coomnibig s t Q.
+Proof using.
+  introv M. induction M; try solve [ constructors* ].
+Qed.
+
+
+(* ########################################################### *)
+(** ** Properties of Coinductive Omni-Big-Step *)
+
+(** [coomnibi] is covariant. *)
 
 Lemma coomnibig_conseq : forall s t Q1 Q2,
   coomnibig s t Q1 ->
@@ -490,72 +512,18 @@ Qed.
 
 
 (* ########################################################### *)
-(** ** From Total to Partial Correctness *)
-
-(** Total correctness is a stronger property than partial correctness:
-    [omnibig s t Q] entails [coomnibig s t Q]. *)
-
-Lemma coomnibig_of_omnibig : forall s t Q,
-  omnibig s t Q ->
-  coomnibig s t Q.
-Proof using.
-  introv M. induction M; try solve [ constructors* ].
-Qed.
-
-
-(* ########################################################### *)
-(** ** Interpretation of Coinductive Omni-Big-Step w.r.t. [safe] *)
-
-(** The predicate [safe s t] asserts that an execution of the configuration
-    [t/s] can never get stuck. Its definition is a simplified version of
-    [coomnibig] where all occurences of [Q] are removed. In the rule for let-
-    bindings, namely [safe_let], the quantification over the configuration
-    [v1/s2] is done by refering to the big-step judgment [eval]. *)
-
-CoInductive safe : state -> trm -> Prop :=
-  | safe_val : forall s v,
-      safe s (trm_val v)
-  | safe_fix : forall s f x t1,
-      safe s (trm_fix f x t1)
-  | safe_app_fix : forall s v1 v2 f x t1,
-      v1 = val_fix f x t1 ->
-      safe s (subst x v2 (subst f v1 t1)) ->
-      safe s (trm_app v1 v2)
-  | safe_let : forall s x t1 t2,
-      safe s t1 ->
-      (forall v1 s2, big s t1 s2 v1 -> safe s2 (subst x v1 t2)) ->
-      safe s (trm_let x t1 t2)
-  | safe_if : forall s b t1 t2,
-      safe s (if b then t1 else t2) ->
-      safe s (trm_if (val_bool b) t1 t2)
-  | safes_div : forall s n1 n2,
-      n2 <> 0 ->
-      safe s (val_div (val_int n1) (val_int n2))
-  | safe_rand : forall s n,
-      n > 0 ->
-      safe s (val_rand (val_int n))
-  | safe_ref : forall s v,
-      safe s (val_ref v)
-  | safe_get : forall s p,
-      Fmap.indom s p ->
-      safe s (val_get (val_loc p))
-  | safe_set : forall s p v,
-      Fmap.indom s p ->
-      safe s (val_set (val_loc p) v)
-  | safe_free : forall s p,
-      Fmap.indom s p ->
-      safe s (val_free (val_loc p)).
+(** ** Coinductive Omni-Big-Step Characterizes Safety and Correctness *)
 
 Section EvalnpSafe.
 Hint Constructors big coomnibig.
 
-(** We prove that [coomnibig s t Q] is equivalent to the conjunction of [safe s t]
+(** We prove that [coomnibig s t Q] is equivalent to the conjunction of [bigsafe s t]
     and to a partial correctness result asserting that if an evaluation of
-    [t/s] terminates on a particular result, then this result satisfies [Q].
-    omni-cobig-iff-safe-and-correct *)
+    [t/s] bigterminates on a particular result, then this result satisfies [Q].
+    omni-cobig-iff-bigsafe-and-correct *)
 
-Lemma coomnibig_iff_safe_and_post : forall s t Q,
-  coomnibig s t Q <-> (safe s t /\ (forall v s', big s t s' v -> Q v s')).
+Lemma coomnibig_iff_bigsafe_and_post : forall s t Q,
+  coomnibig s t Q <-> (bigsafe s t /\ (forall v s', big s t s' v -> Q v s')).
 Proof using.
   iff M.
   { split.
@@ -574,48 +542,27 @@ Proof using.
         { introv R2. applys* HQ. } } } }
 Qed.
 
-(** We prove that [safe s t] is equivalent to [coomnibig s t Any]. *)
+(** We prove that [coomnibig s t Any] is equivalent to [bigsafe s t]. *)
 
-Lemma safe_iff_coomnibig_any : forall s t,
-  safe s t <-> coomnibig s t Any.
+Lemma bigsafe_iff_coomnibig_any : forall s t,
+  coomnibig s t Any <-> bigsafe s t.
 Proof using.
-  intros. rewrite* (coomnibig_iff_safe_and_post s t Any).
+  intros. rewrite* (coomnibig_iff_bigsafe_and_post s t Any).
 Qed.
 
 End EvalnpSafe.
 
 
-
 (* ########################################################### *)
 (* ########################################################### *)
 (* ########################################################### *)
-(** * Characterization of Divergence *)
-
-(** We present several characterization of divergence and prove
-    them equivalent. *)
+(** * Remarks *)
 
 
 (* ########################################################### *)
-(** ** Omni-Big-Step Divergence *)
-
-(** The judgment [coomnidiv s t] asserts that every possible
-    execution of the program [(s,t)] diverges. It is defined
-    in terms of the coinductive Omni-big-step judgment. *)
-
-Definition coomnidiv (s:state) (t:trm) : Prop :=
-  coomnibig s t Empty.
-
-
-
-(* ########################################################### *)
-(* ########################################################### *)
-(* ########################################################### *)
-(** * Beyond A-normal form: Adding the Bind Rule  *)
+(** ** Omni-Big-Step Judgment with the Bind Rule *)
 
 Module Bind.
-
-(* ########################################################### *)
-(** ** Omni-Big-Step Judgment with Evaluation under Context *)
 
 (** Definition of evaluation contexts *)
 
@@ -700,6 +647,28 @@ Proof using.
   induction M; try solve [ constructors* ].
 Qed.
 
+(** Frame property for [omnibig s t Q], expressed using the
+    separation logic star operator. *)
+
+Implicit Types h : state.
+
+Definition hstar (H1 H2 : hprop) : hprop :=
+  fun h => exists h1 h2, H1 h1 /\ H2 h2 /\ Fmap.disjoint h1 h2 /\ h = h1 \u h2.
+
+Notation "H1 '\*' H2" := (hstar H1 H2) (at level 41, right associativity).
+
+Lemma hstar_intro : forall H1 H2 h1 h2,
+  H1 h1 ->
+  H2 h2 ->
+  Fmap.disjoint h1 h2 ->
+  (H1 \* H2) (h1 \u h2).
+Proof using. intros. exists* h1 h2. Qed.
+
+Lemma hstar_inv : forall H1 H2 h,
+  (H1 \* H2) h ->
+  exists h1 h2, H1 h1 /\ H2 h2 /\ Fmap.disjoint h1 h2 /\ h = h1 \u h2.
+Proof using. introv M. hnf in M. jauto. Qed.
+
 Lemma omnibig_frame : forall h1 h2 t Q,
   omnibig h1 t Q ->
   Fmap.disjoint h1 h2 ->
@@ -724,59 +693,15 @@ Proof using.
       { auto. } { auto. } { applys* Fmap.disjoint_remove_l. } } }
 Qed.
 
-
-
-
-
-(* ########################################################### *)
-(* ########################################################### *)
-(** * Compiler Correctness For Terminating Programs *)
-
-Section CompilerCorrectnessTerminating.
-
-(** Consider a compilation function. For simplicity, we assume
-    here that the corresponding compilation phase does not affect
-    the memory state during program executions (this is in particular
-    the case for compilation of purely functional programs). *)
-
-Parameter compile : trm -> trm.
-
-(** Assume that it satisfies Omni-forward-preservation. *)
-
-Parameter omni_forward_preservation_for_compile : forall s t Q,
-  omnibig s t Q ->
-  omnibig s (compile t) Q.
-
-(** We show that Omni-forward-preservation entails correctness
-    for terminating programs. *)
-
-Lemma compile_correct : forall s t,
-  terminates s t ->
-     terminates s (compile t)
-  /\ (forall s' v, big s (compile t) s' v -> big s t s' v).
-Proof using.
-  introv HT.
-  forwards R: omni_forward_preservation_for_compile s t (strongestpost s t).
-  { applys omnibig_strongestpost_of_terminates HT. }
-  split.
-  { applys terminates_of_omnibig R. }
-  { introv M. applys omnibig_and_big_inv R M. }
-Qed.
-
-End CompilerCorrectnessTerminating.
-
-
+End Bind.
 
 
 (* ########################################################### *)
-(* ########################################################### *)
-(* ########################################################### *)
-(** * Inductive PRECISE-Omni-Big-Step  *)
+(** ** Definition of Precise Omni-semantics *)
 
-(* ########################################################### *)
-(** ** Definition of precise Omni-semantics *)
-
-(** Judgment [pomnibig s t Q] with precise outcome *)
+(** Judgment [pomnibig s t Q] asserts that all executions of [(s,t)]
+    are safe and terminating, and the set of possible final configurations
+    is described exactly by [Q]. *)
 
 Inductive pomnibig : state -> trm -> (val->state->Prop) -> Prop :=
   | pomnibig_val : forall s v Q,
@@ -799,7 +724,7 @@ Inductive pomnibig : state -> trm -> (val->state->Prop) -> Prop :=
       pomnibig s (trm_if (val_bool b) t1 t2) Q
   | pomnibig_div : forall s n1 n2 Q,
       n2 <> 0 ->
-      Q (val_int (Z.quot n1 n2)) s ->
+      Q = exactly (Z.quot n1 n2) s ->
       pomnibig s (val_div (val_int n1) (val_int n2)) Q
   | pomnibig_rand : forall s n Q (Qof:int->val->hprop),
       n > 0 ->
@@ -824,13 +749,10 @@ Inductive pomnibig : state -> trm -> (val->state->Prop) -> Prop :=
       Q = exactly val_unit (Fmap.remove s p) ->
       pomnibig s (val_free (val_loc p)) Q.
 
-
-(* ########################################################### *)
-(** ** Properties of precise Omni-semantics *)
-
 (** [pomnibig s t Q] relates a program with exactly the set [Q]
     that corresponds exactly to the set of possible results,
-    no more, no less. *)
+    no more, no less. Thus, [Q] must correspond to the strongest
+    postcondition of the configuration [(s,t)]. *)
 
 Lemma pomnibig_characterizes_strongestpost : forall s t Q,
   pomnibig s t Q ->
@@ -849,8 +771,8 @@ Proof using.
     { inverts M1 as R1 R2. exists. split*. rewrite* K. } }
   { subst. extens; intros v' s'. unfold strongestpost. iff M1.
     { applys* big_if. } { inverts* M1. } }
-  { subst. extens; intros v' s'. unfold exactly, strongestpost.
-    iff (->&->) M1. { constructors*. } { inverts* M1. } }
+  { subst. extens; intros v' s'. unfold strongestpost.
+    iff (->&->) M1. { constructors*. } { inverts* M1. splits*. } }
   { rename H0 into K.
     subst. extens; intros v' s'. unfold exactly, strongestpost.
     iff (n1&E1&R1) M1.
@@ -869,8 +791,8 @@ Proof using.
     iff (->&->) M1. { constructors*. } { inverts M1; tryfalse. auto. } }
 Qed.
 
-(** Assume [pomnibig s t Q] to hold. Prove that the postcondition [Q] holds of
-    any output that [(s,t)] may evaluate to according to the judgment [big]. *)
+(** Assume [pomnibig s t Q] to hold. We can prove that the postcondition [Q] holds
+    of any output that [(s,t)] may evaluate to according to the judgment [big]. *)
 
 Lemma pomnibig_and_big_inv : forall s t v s' Q,
   pomnibig s t Q ->
@@ -881,9 +803,9 @@ Proof using.
   rewrite E. apply R.
 Qed.
 
-(** If [pomnibig s t Q] holds, then there exists an output
-    [(s',v)] that [(s,t)] may evaluate to according to the judgment
-    [big], and that this output satisfies [Q]. *)
+(** If [pomnibig s t Q] holds, then there exists at least one final
+    configuration [(s',v)] such that [(s,t)] evaluates to this configuration
+    according to the judgment [big]; moreover this output satisfies [Q]. *)
 
 Lemma pomnibig_to_one_big : forall s t Q,
   pomnibig s t Q ->
@@ -914,24 +836,29 @@ Proof using.
   { exists. applys* big_free. }
 Qed.
 
-(** Auxilary lemma for the next proof *)
-Lemma strongestpost_eq_exactly : forall s t v,
+(** An auxilary lemma for the next proof. *)
+
+Lemma strongestpost_one : forall s t v,
   (forall v' s', big s t s' v' <-> v' = v /\ s' = s) ->
   strongestpost s t = exactly v s.
 Proof using.
   introv M. unfold strongestpost, exactly. extens*.
 Qed.
 
-(** If a term is safe according to [omnibig], which overapproximates
-    the set of results, then [pcpbig], which is precise, holds. *)
+(** If the configuration [(s,t)] satisfies [omnibig] for a postcondition
+    [Q], then it implies that all executions of [(s,t)] are bigsafe.
+    It follows that [pomnibig] holds of that configuration, for the
+    postcondition equal to [strongestpost s t]. This lemma is related
+    to [omnibig_inv_strongestpost_qimpl]. *)
+
 Lemma pomnibig_of_omnibig : forall s t Q,
   omnibig s t Q ->
   pomnibig s t (strongestpost s t).
 Proof using.
   hint exactly_intro. introv M. induction M.
-  { constructors. applys strongestpost_eq_exactly.
+  { constructors. applys strongestpost_one.
    intros. iff R (->&->). { inverts* R. } { constructors*. } }
-  { constructors. applys strongestpost_eq_exactly.
+  { constructors. applys strongestpost_one.
     intros. iff R (->&->). { inverts* R. } { constructors*. } }
   { applys* pomnibig_app_fix. applys_eq IHM. extens.
     unfold strongestpost. intros v' s'. iff R.
@@ -944,7 +871,7 @@ Proof using.
       { inverts* R. } { constructors*. } } }
   { constructors. applys_eq IHM. extens. unfold strongestpost.
     intros v' s'. iff R. { inverts* R. } { constructors*. } }
-  { constructors. applys strongestpost_eq_exactly.
+  { constructors*. applys strongestpost_one.
     intros. iff R (->&->). { inverts* R. } { constructors*. } }
   { applys* pomnibig_rand. simpl. unfold strongestpost. extens.
     intros v' s'. iff R (?&?&(->&->)). { inverts R; tryfalse. exists* n1. }
@@ -952,7 +879,7 @@ Proof using.
   { applys* pomnibig_ref. simpl. unfold strongestpost. extens.
     intros v' s'. iff R (?&?&(->&->)). { inverts R; tryfalse. exists* p. }
     { applys* big_ref. } }
-  { constructors*. applys strongestpost_eq_exactly.
+  { constructors*. applys strongestpost_one.
     intros. iff R (->&->). { inverts R; tryfalse; eauto. } { constructors*. } }
   { constructors*. unfold strongestpost, exactly. extens*.
     intros v' s'. iff R (->&->). { inverts R; tryfalse; eauto. } { constructors*. } }
@@ -960,6 +887,96 @@ Proof using.
     intros v' s'. iff R (->&->). { inverts R; tryfalse; eauto. } { constructors*. } }
 Qed.
 
-(** See also [omnibig_inv_strongestpost_qimpl], which asserts that
-    if [omnibig s t Q], then [Q] contains [strongestpost s t]. *)
 
+(* ########################################################### *)
+(** ** Relationship with WP Formulation *)
+
+(** The rule [omnibig_let] shares similarities with the statement of
+    the weakest-precondition style reasoning rule for let-bindings.
+    Prove the following alternative statement, with a wp-style flavor. *)
+
+Lemma omnibig_let' : forall s1 x t1 t2 Q,
+  omnibig s1 t1 (fun v1 s2 => omnibig s2 (subst x v1 t2) Q) ->
+  omnibig s1 (trm_let x t1 t2) Q.
+Proof using.
+  introv M. applys* omnibig_let M.
+Qed.
+
+(** Reciprocally, prove that the statement considered in the inductive
+    definition of [omnibig] is derivable from [omnibig_let']. More precisely,
+    prove the statement below by using [omnibig_let'] and [omnibig_conseq]. *)
+
+Lemma omnibig_let_of_omnibig_let' : forall Q1 s1 x t1 t2 Q,
+  omnibig s1 t1 Q1 ->
+  (forall v1 s2, Q1 v1 s2 -> omnibig s2 (subst x v1 t2) Q) ->
+  omnibig s1 (trm_let x t1 t2) Q.
+Proof using.
+  introv M1 M2. applys omnibig_let'. applys omnibig_conseq M1.
+  intros v1 s2 K. applys M2 K.
+Qed.
+
+(** One way wonder whether we could have used the wp-style formulation
+    of the semantics of let-bindings directly in the definition of [omnibig].
+    The answer is negative. Doing so would lead to an invalid inductive
+    definition, involving a "non strictly positive occurrence". To check it
+    out, uncomment the definitions below to observe Coq's complaint.
+[[
+  Inductive omnibig' : state -> trm -> (val->state->Prop) -> Prop :=
+    | omnibig'_let : forall s1 x t1 t2 Q,
+       omnibig' s1 t1 (fun v1 s2 => omnibig' s2 (subst x v1 t2) Q) ->
+       omnibig' s1 (trm_let x t1 t2) Q.
+
+  Inductive omnibig' : state -> trm -> (val->state->Prop) -> Prop :=
+    | omnibig'_let : forall Q1 s1 x t1 t2 Q,
+       omnibig' s1 t1 Q1 ->
+       Q1 = (fun v1 s2 => omnibig' s2 (subst x v1 t2) Q) ->
+       omnibig' s1 (trm_let x t1 t2) Q.
+]]
+
+   Yet another unsuccessful try:
+[[
+  Inductive omnibig' : state -> trm -> (val->state->Prop) -> Prop :=
+    | omnibig'_let : forall Q1 s1 x t1 t2 Q,
+       omnibig' s1 t1 Q1 ->
+       (forall v1 s2, Q1 v1 s2 -> exists Q2, omnibig' s2 (subst x v1 t2) Q2) ->
+       Q = (fun v2 s3 => exists v1 s2, Q1 v1 s2 /\ exists Q2, Q2 v2 s3 /\ omnibig' s2 (subst x v1 t2) Q2) ->
+       omnibig' s1 (trm_let x t1 t2) Q.
+]]
+*)
+
+
+(* ########################################################### *)
+(** ** Compiler Correctness For Terminating Programs *)
+
+Section CompilerCorrectnessTerminating.
+
+(** Consider a compilation function. For simplicity, we assume
+    here that the corresponding compilation phase does not affect
+    the memory state during program executions (this is in particular
+    the case for compilation of purely functional programs). *)
+
+Parameter compile : trm -> trm.
+
+(** Assume that it satisfies Omni-forward-preservation. *)
+
+Parameter omni_forward_preservation_for_compile : forall s t Q,
+  omnibig s t Q ->
+  omnibig s (compile t) Q.
+
+(** We show that Omni-forward-preservation entails correctness
+    for terminating programs. *)
+
+Lemma compile_correct : forall s t,
+  bigterminates s t ->
+     bigterminates s (compile t)
+  /\ (forall s' v, big s (compile t) s' v -> big s t s' v).
+Proof using.
+  introv HT.
+  forwards R: omni_forward_preservation_for_compile s t (strongestpost s t).
+  { applys omnibig_strongestpost_of_bigterminates HT. }
+  split.
+  { applys bigterminates_of_omnibig R. }
+  { introv M. applys omnibig_and_big_inv R M. }
+Qed.
+
+End CompilerCorrectnessTerminating.
