omni/Big.v
@@ -91,3 +91,4 @@ CoInductive codiv : state -> trm -> Prop :=
     Coinductive big-step operational semantics,
     Xavier Leroy and Hervé Grall, ESOP 2006,
     https://xavierleroy.org/coindsem/ *)
+
