omni/EquivOmni.v
@@ -10,8 +10,8 @@ Require Export Syntax.
 (* ########################################################### *)
 (** ** Equivalence Between Eventually and Omni-Big-Step Semantics *)
 
-(** We start by establishing the equivalence between [bigsmall] and [omnibig].
-    We focus first on the direction from [bigsmall] to [omnibig]. *)
+(** We start by establishing the equivalence between [stepsinto] and [omnibig].
+    We focus first on the direction from [stepsinto] to [omnibig]. *)
 
 (** We begin with a key lemma: if a configuration [(s1,t1)] takes a step to
     [(s2,t2)], then this first configuration admits the same postconditions
@@ -54,10 +54,10 @@ Proof using.
 Qed.
 
 (** By exploiting the above lemma over all the steps of an execution, we obtain
-    the fact that [bigsmall] implies [omnibig]. *)
+    the fact that [stepsinto] implies [omnibig]. *)
 
-Lemma omnibig_of_bigsmall : forall s t Q,
-  bigsmall s t Q ->
+Lemma omnibig_of_stepsinto : forall s t Q,
+  stepsinto s t Q ->
   omnibig s t Q.
 Proof using.
   introv M. induction M.
@@ -65,21 +65,21 @@ Proof using.
   { applys* omnibig_of_step_and_omnibig. }
 Qed.
 
-(** Let's now turn to the second direction, from [omnibig] to [bigsmall].
-    We first need an introduction lemma for let-bindings for [bigsmall]. *)
+(** Let's now turn to the second direction, from [omnibig] to [stepsinto].
+    We first need an introduction lemma for let-bindings for [stepsinto]. *)
 
-Lemma bigsmall_let : forall s x t1 t2 Q1 Q,
-  bigsmall s t1 Q1 ->
-  (forall s1 v1, Q1 v1 s1 -> bigsmall s1 (subst x v1 t2) Q) ->
-  bigsmall s (trm_let x t1 t2) Q.
+Lemma stepsinto_let : forall s x t1 t2 Q1 Q,
+  stepsinto s t1 Q1 ->
+  (forall s1 v1, Q1 v1 s1 -> stepsinto s1 (subst x v1 t2) Q) ->
+  stepsinto s (trm_let x t1 t2) Q.
 Proof using.
   introv M1 M2. gen_eq Q1': Q1.
   induction M1; intros; subst.
-  { apply bigsmall_step.
+  { apply stepsinto_step.
     { do 2 esplit. applys step_let. }
     { introv R. inverts R as R'. { inverts R'. } applys* M2. } }
   { rename t into t1, H1 into IH.
-    destruct H as (s'&t'&RE). applys bigsmall_step.
+    destruct H as (s'&t'&RE). applys stepsinto_step.
     { do 2 esplit. constructors. applys RE. }
     { introv R. inverts R as R'.
       { applys* IH R' M2. }
@@ -88,68 +88,68 @@ Qed.
 
 (** The proof is carried out by induction on the big-step relation. *)
 
-Lemma bigsmall_of_omnibig : forall s t Q,
+Lemma stepsinto_of_omnibig : forall s t Q,
   omnibig s t Q ->
-  bigsmall s t Q.
+  stepsinto s t Q.
 Proof using.
   introv M. induction M.
-  { applys* bigsmall_val. }
-  { applys bigsmall_step.
+  { applys* stepsinto_val. }
+  { applys stepsinto_step.
     { do 2 esplit. applys step_fix. }
-    { introv K. inverts K. applys* bigsmall_val. } }
-  { rename H into E. applys bigsmall_step.
+    { introv K. inverts K. applys* stepsinto_val. } }
+  { rename H into E. applys stepsinto_step.
     { do 2 esplit. applys* step_app_fix. }
     { introv K. invert K; try solve [ intros; false ].
       introv -> -> -> -> -> R. inverts E. applys IHM. } }
   { rename M into M1, H into M2, IHM into IHM1, H0 into IHM2.
     tests C: (exists v1, t1 = trm_val v1).
-    { destruct C as (v1&->). applys bigsmall_step.
+    { destruct C as (v1&->). applys stepsinto_step.
       { do 2 esplit. applys* step_let. }
       { introv K. inverts K as K1 K2.
         { inverts K1. }
         { inverts IHM1 as K3 K4.
           { applys* IHM2. }
           { destruct K3 as (?&?&K5). inverts K5. } } } }
-    { applys bigsmall_step.
+    { applys stepsinto_step.
       { inverts IHM1 as K3 K4.
         { false* C. }
         { destruct K3 as (?&?&K5). do 2 esplit. applys* step_let_ctx. } }
       { introv K. inverts K as K'; [|false* C].
         inverts IHM1 as K5 K6; [false* C|].
-        specializes K6 K'. applys* bigsmall_let. } } }
-  { applys bigsmall_step.
+        specializes K6 K'. applys* stepsinto_let. } } }
+  { applys stepsinto_step.
     { do 2 esplit. applys* step_if. }
     { introv K. inverts K. applys IHM. } }
-  { applys bigsmall_step.
+  { applys stepsinto_step.
     { do 2 esplit. applys* step_div. }
-    { introv K. inverts K. applys* bigsmall_val. } }
-  { applys bigsmall_step.
+    { introv K. inverts K. applys* stepsinto_val. } }
+  { applys stepsinto_step.
     { do 2 esplit. applys* step_rand 0. math. }
-    { introv K. inverts K; tryfalse. applys* bigsmall_val. } }
-  { applys bigsmall_step.
+    { introv K. inverts K; tryfalse. applys* stepsinto_val. } }
+  { applys stepsinto_step.
     { forwards~ (p&D&N): (exists_fresh null s).
       do 2 esplit. applys* step_ref. }
-    { introv K. inverts K; tryfalse. applys* bigsmall_val. } }
-  { applys bigsmall_step.
+    { introv K. inverts K; tryfalse. applys* stepsinto_val. } }
+  { applys stepsinto_step.
     { do 2 esplit. applys* step_get. }
-    { introv K. inverts K; tryfalse. applys* bigsmall_val. } }
-  { applys bigsmall_step.
+    { introv K. inverts K; tryfalse. applys* stepsinto_val. } }
+  { applys stepsinto_step.
     { do 2 esplit. applys* step_set. }
-    { introv K. inverts K; tryfalse. applys* bigsmall_val. } }
-  { applys bigsmall_step.
+    { introv K. inverts K; tryfalse. applys* stepsinto_val. } }
+  { applys stepsinto_step.
     { do 2 esplit. applys* step_free. }
-    { introv K. inverts K; tryfalse. applys* bigsmall_val. } }
+    { introv K. inverts K; tryfalse. applys* stepsinto_val. } }
 Qed.
 
 (** Combining the two directions, we obtain the desired equivalence between
     omni-big-step and inductive-small-step. *)
 
-Lemma bigsmall_eq_omnibig :
-  bigsmall = omnibig.
+Lemma stepsinto_eq_omnibig :
+  stepsinto = omnibig.
 Proof using.
   extens. intros s t Q. iff M.
-  { applys* omnibig_of_bigsmall. }
-  { applys* bigsmall_of_omnibig. }
+  { applys* omnibig_of_stepsinto. }
+  { applys* stepsinto_of_omnibig. }
 Qed.
 
 (** The final equivalence follows. *)
@@ -157,8 +157,8 @@ Qed.
 Lemma omnibig_iff_eventually : forall s t Q,
   omnibig s t Q <-> eventually s t (pred_of_post Q).
 Proof using.
-  intros. rewrite <- bigsmall_eq_omnibig.
-  rewrite* bigsmall_iff_eventually.
+  intros. rewrite <- stepsinto_eq_omnibig.
+  rewrite* stepsinto_iff_eventually.
 Qed.
 
 
@@ -166,22 +166,22 @@ Qed.
 (* ########################################################### *)
 (** ** Equivalence Between CoInductive Big-Step and Standard Partial Correctness *)
 
-(** The first step of the proof is to formally relate [cobigsmall]
+(** The first step of the proof is to formally relate [costepsinto]
    and [coomnibig], which are both defined coinductively. *)
 
-(** The first direction is from [cobigsmall] to [coomnibig].
+(** The first direction is from [costepsinto] to [coomnibig].
     To establish it, we need inversion lemmas for let-bindings. *)
 
-Lemma cobigsmall_let_inv_ctx : forall x s1 t1 t2 Q Q1,
-  cobigsmall s1 (trm_let x t1 t2) Q ->
+Lemma costepsinto_let_inv_ctx : forall x s1 t1 t2 Q Q1,
+  costepsinto s1 (trm_let x t1 t2) Q ->
   (fun v s => steps s1 t1 s v) ===> Q1 ->
-  cobigsmall s1 t1 Q1.
+  costepsinto s1 t1 Q1.
 Proof using.
   cofix IH. introv M WQ. inverts M as M0 M'.
   tests C: (exists v1, t1 = trm_val v1).
-  { destruct C as (v1&->). applys cobigsmall_val.
+  { destruct C as (v1&->). applys costepsinto_val.
     applys WQ. applys steps_refl. }
-  { applys cobigsmall_step.
+  { applys costepsinto_step.
     { destruct M0 as (s'&t'&S). inverts S as. 2:{ false* C. }
       intros S. exists. applys S. }
     { intros s2 t1' S. applys IH.
@@ -189,10 +189,10 @@ Proof using.
       { intros v s R. applys WQ. applys steps_step S R. } } }
 Qed.
 
-Lemma cobigsmall_let_inv_cont : forall s1 s2 v1 x t1 t2 Q,
-  cobigsmall s1 (trm_let x t1 t2) Q ->
+Lemma costepsinto_let_inv_cont : forall s1 s2 v1 x t1 t2 Q,
+  costepsinto s1 (trm_let x t1 t2) Q ->
   steps s1 t1 s2 v1 ->
-  cobigsmall s2 (subst x v1 t2) Q.
+  costepsinto s2 (subst x v1 t2) Q.
 Proof using.
   introv M R. gen_eq t1': (trm_val v1). induction R; intros; subst.
   { inverts M as _ M'. applys M'. applys step_let. }
@@ -201,21 +201,21 @@ Proof using.
     applys step_let_ctx S. }
 Qed.
 
-Lemma cobigsmall_let_inv : forall s1 x t1 t2 Q,
-  cobigsmall s1 (trm_let x t1 t2) Q ->
-  exists Q1, cobigsmall s1 t1 Q1
-          /\ (forall v1 s2, Q1 v1 s2 -> cobigsmall s2 (subst x v1 t2) Q).
+Lemma costepsinto_let_inv : forall s1 x t1 t2 Q,
+  costepsinto s1 (trm_let x t1 t2) Q ->
+  exists Q1, costepsinto s1 t1 Q1
+          /\ (forall v1 s2, Q1 v1 s2 -> costepsinto s2 (subst x v1 t2) Q).
 Proof using.
   introv M. exists (fun v s => steps s1 t1 s (trm_val v)). split.
-  { applys* cobigsmall_let_inv_ctx M. }
-  { introv K. applys* cobigsmall_let_inv_cont M K. }
+  { applys* costepsinto_let_inv_ctx M. }
+  { introv K. applys* costepsinto_let_inv_cont M K. }
 Qed.
 
 (** Using these inversion lemmas, we can prove by induction the first
-    direction, from [cobigsmall] to [coomnibig]. *)
+    direction, from [costepsinto] to [coomnibig]. *)
 
-Lemma coomnibig_of_cobigsmall : forall s t Q,
-  cobigsmall s t Q ->
+Lemma coomnibig_of_costepsinto : forall s t Q,
+  costepsinto s t Q ->
   coomnibig s t Q.
 Proof using.
   cofix IH. introv M. destruct t; try solve [ inverts M; false_invert ].
@@ -251,7 +251,7 @@ Proof using.
     { introv D. applys* coomnibig_free.
       forwards M1': M1. { applys* step_free. }
       inverts M1' as. { auto. } { intros. false* exists_step_val_inv. } } }
-  { lets (Q1&M1&M2): cobigsmall_let_inv M. applys coomnibig_let.
+  { lets (Q1&M1&M2): costepsinto_let_inv M. applys coomnibig_let.
     { applys IH. applys M1. }
     { introv R. applys IH. applys M2 R. } }
   { inverts M as (s'&t'&S) M1. inverts S. applys coomnibig_if.
@@ -261,7 +261,7 @@ Qed.
 (** For the reciprocal direction, we also need one key inversion lemma. It
     is stated below. Its hypothesis is [coomnibig s t Q], and its conclusion
     corresponds to the disjunction of the constructors of the inductive
-    definition of [cobigsmall s t Q]. *)
+    definition of [costepsinto s t Q]. *)
 
 Lemma coomnibig_inv_step : forall s t Q,
   coomnibig s t Q ->
@@ -314,29 +314,29 @@ Proof using.
 Qed.
 
 (** Using this inversion lemma, it is straightforward to derive the
-    implication from [coomnibig] to [cobigsmall]. *)
+    implication from [coomnibig] to [costepsinto]. *)
 
-Lemma cobigsmall_of_coeval : forall s t Q,
+Lemma costepsinto_of_coeval : forall s t Q,
   coomnibig s t Q ->
-  cobigsmall s t Q.
+  costepsinto s t Q.
 Proof.
   cofix IH. introv M. lets C: coomnibig_inv_step M.
   destruct C as [(v&->&HQ)|((s'&t'&S&M1)&M2)].
-  { applys cobigsmall_val HQ. }
-  { applys cobigsmall_step.
+  { applys costepsinto_val HQ. }
+  { applys costepsinto_step.
     { exists. applys S. }
     { intros s1 t1 S'. applys IH. applys M2 S'. } }
 Qed.
 
-(** Combining the two directions yields the equality between [cobigsmall] and
+(** Combining the two directions yields the equality between [costepsinto] and
     [coomnibig], and that between [partial] and [coomnibig]. *)
 
-Lemma cobigsmall_eq_omnibigp :
-   cobigsmall = coomnibig.
+Lemma costepsinto_eq_omnibigp :
+   costepsinto = coomnibig.
 Proof using.
   extens. intros s t Q. iff M.
-  { applys* coomnibig_of_cobigsmall. }
-  { applys* cobigsmall_of_coeval. }
+  { applys* coomnibig_of_costepsinto. }
+  { applys* costepsinto_of_coeval. }
 Qed.
 
 (** Finally, we conclude that coinductive Omni-big-step matches the
@@ -345,7 +345,7 @@ Qed.
 Lemma coomnibig_eq_partial :
   coomnibig = partial.
 Proof using.
-  rewrite <- cobigsmall_eq_partial. rewrite* cobigsmall_eq_omnibigp.
+  rewrite <- costepsinto_eq_partial. rewrite* costepsinto_eq_omnibigp.
 Qed.
 
 
@@ -388,8 +388,8 @@ Lemma sdiv_eq_coomnidiv :
 Proof using.
   extens. intros s t. unfold coomnidiv.
   rewrite sdiv_iff_omnibigps_Empty.
-  rewrite <- cobigsmall_eq_omnibigp.
-  rewrite* cobigsmall_eq_partial.
+  rewrite <- costepsinto_eq_omnibigp.
+  rewrite* costepsinto_eq_partial.
 Qed.
 
 
@@ -453,11 +453,32 @@ End OmnismallEquiv.
 
 
 
+(** [eventually] is equivalent to [seventually]. *)
+
+Lemma eventually_eq_seventually :
+  eventually = seventually.
+Proof using.
+  extens. intros s t P. iff M.
+  { induction M.
+    { applys* seventually_here. }
+    { rename H into M1, H0 into M2, H1 into IHM2.
+      rewrite omnismall_iff_step_st in M1. destruct M1 as (R&M1).
+      applys* seventually_step R. } }
+  { induction M.
+    { applys* eventually_here. }
+    { rename H into R, H0 into M1, H1 into IHM1.
+      applys eventually_step (step s t).
+      { rewrite omnismall_iff_step_st. split*. }
+      { autos*. } } }
+Qed.
+
+
+
 
 (* ########################################################### *)
 (** ** Inductive Small-Step Judgment *)
 
-(** The judgment [bigsmall] introduced in this section helps
+(** The judgment [stepsinto] introduced in this section helps
     carrying out several proofs of equivalence---see the next
     section. *)
 
@@ -469,21 +490,21 @@ Definition pred_of_post (Q:val->hprop) : state->trm->Prop :=
 (** We introduce the inductive small-step judgment, as it is useful
     to relate Omni-Small-Step with Omni-Big-Step.
 
-(** [bigsmall] is equivalent to [eventually]. *)
+(** [stepsinto] is equivalent to [eventually]. *)
 
-Lemma bigsmall_iff_eventually : forall s t Q,
-  bigsmall s t Q <-> eventually s t (pred_of_post Q).
+Lemma stepsinto_iff_eventually : forall s t Q,
+  stepsinto s t Q <-> eventually s t (pred_of_post Q).
 Proof using.
-  rewrite eventually_eq_eventually'.
+  rewrite eventually_eq_seventually.
   iff M.
   { induction M.
-    { applys eventually'_here. hnf. exists*. }
+    { applys seventually_here. hnf. exists*. }
     { rename H into R, H0 into M1, H1 into IH1.
-      applys eventually'_step R. applys IH1. } }
+      applys seventually_step R. applys IH1. } }
   { gen_eq C: (pred_of_post Q). induction M; intros; subst.
-    { destruct H as (v'&->&Hv'). applys bigsmall_val Hv'. }
+    { destruct H as (v'&->&Hv'). applys stepsinto_val Hv'. }
     { rename H into R, H0 into M1, H1 into IH1.
-      applys bigsmall_step R.
+      applys stepsinto_step R.
       intros s' t' S. applys* IH1 S. } }
 Qed.
 
